pcuic/theories/PCUICWeakening.v
@@ -1055,16 +1055,14 @@ Proof.
       now specialize (Hs' _ _ _ wf eq_refl).
     * eapply All_map.
       eapply (All_impl X1); simpl.
-      intros x [[Hb Hlam] IH].
+      intros x [Hb IH].
       rewrite lift_fix_context.
       specialize (IH Γ (Γ' ,,,  (fix_context mfix)) Γ'' wf).
       rewrite app_context_assoc in IH. specialize (IH eq_refl).
-      split; auto.
-      + rewrite lift_context_app Nat.add_0_r app_context_assoc in IH.
-        rewrite app_context_length fix_context_length in IH.
-        rewrite lift_context_length fix_context_length.
-        rewrite permute_lift; try lia. now rewrite (Nat.add_comm #|Γ'|).
-      + now rewrite isLambda_lift.
+      rewrite lift_context_app Nat.add_0_r app_context_assoc in IH.
+      rewrite app_context_length fix_context_length in IH.
+      rewrite lift_context_length fix_context_length.
+      rewrite permute_lift; try lia. now rewrite (Nat.add_comm #|Γ'|).
     * red; rewrite <-H1. unfold wf_fixpoint.
       rewrite map_map_compose.
       now rewrite weakening_check_one_fix.
